Escallon/LR_Parsing/Generalized_Pushdown_Automata.thy
@@ -9,11 +9,6 @@ record ('q, 'a) gpda = states :: "'q set"
                        final  :: "'q set"
                        nxt    :: "('q list \<times> 'a \<times> 'q list) set"
                        eps    :: "('q list \<times> 'q list) set"
-                      
-(* Placeholder, should be states M 
-consts Q :: "'s::fresh0 set" 
-
-*)
 
 locale gpda =
   fixes M :: "('q, 'a) gpda"
@@ -24,8 +19,11 @@ locale gpda =
       and eps:        "(ps, qs) \<in> eps M \<Longrightarrow> ps \<noteq> [] \<and> qs \<noteq> [] 
         \<and> set ps \<subseteq> states M \<and> set qs \<subseteq> states M"
       and finite:     "finite (states M)"
+(* 
+  Necessary only for L(GPDA) \<subseteq> L(PDA) to hold. 
       and finite_nxt: "finite (nxt M)"
       and finite_eps: "finite (eps M)"
+*)
 begin
 
 type_synonym ('s, 'b) config = "'s list \<times> 'b list"
@@ -56,6 +54,15 @@ lemma step_states_imp_states:
   shows "set qs \<subseteq> states M"
   using assms nxt eps by cases auto
 
+lemma step_equal_or_Cons:
+  assumes "(p,u) \<turnstile> (q,v)"
+  shows "u = v \<or> (\<exists>a. u = a#v)"
+  using assms by cases auto
+
+lemma step_len_dec:
+  assumes "(p,u) \<turnstile> (q,v)"
+  shows "length u \<ge> length v" 
+  using step_equal_or_Cons[OF assms] by fastforce
 
 abbreviation steps :: "('q,'a) config \<Rightarrow> ('q,'a) config \<Rightarrow> bool" (infix \<open>\<turnstile>*\<close> 55) where
   "steps \<equiv> step\<^sup>*\<^sup>*"
@@ -86,172 +93,8 @@ corollary steps_init_imp_states:
   shows "set qs \<subseteq> states M"
   using steps_states_imp_states[OF assms] init by auto
 
-
 definition Lang :: "'a list set" where
   "Lang \<equiv> {w. \<exists>f \<in> final M. ([init M], w) \<turnstile>* ([f], [])}"
 
-(*
-
-Towards gpda \<Longrightarrow> pda
-
-definition states_of_eps :: "('s list \<times> 's list) set \<Rightarrow> 's set" where
-  "states_of_eps \<E> \<equiv> \<Union>(ps, qs) \<in> \<E>. set ps \<union> set qs"
-
-popwrt_eps should turn 
-
-  ps \<turnstile> qs for ps = p\<^sub>0#p\<^sub>1#...#p\<^sub>n 
-
-into
-
-  p\<^sub>0#p\<^sub>1#...#p\<^sub>n \<turnstile> p\<^sub>1#...#p\<^sub>n \<turnstile> ... \<turnstile> p\<^sub>n \<turnstile> qs
-
-fun popwrt_eps :: "'s set \<Rightarrow> 's list \<Rightarrow> 's list \<Rightarrow> ('s \<times> 's) list" where
-  "popwrt_eps Q qs \<gamma> = undefined"
-
-
-
-definition List_pda :: "('q, 'a, 'q) pda" where
-  "List_pda \<equiv> 
-    \<lparr>pda.init_state = undefined, init_symbol = undefined, final_states = undefined, delta = undefined, delta_eps = undefined\<rparr>"
-
-*)
-
 end
-
-section \<open>Equivalence with PDAs\<close>
-
-datatype ('a, 'b, 'c) sum3 = Qtyp 'a | Styp 'b | Q'typ 'c
-
-definition gpda_of_pda :: "('q, 'a, 's) pda \<Rightarrow> (('q, 's, 'r::fresh0) sum3, 'a) gpda" where
-  "gpda_of_pda M \<equiv> let 
-    Q\<^sub>M = UNIV :: 'q set;
-    \<Gamma> = UNIV :: 's set; 
-    q\<^sub>0 = fresh0 ({}::'r set);
-    q\<^sub>f = fresh0 {q\<^sub>0};
-    \<Delta> = {([Qtyp p, Styp Z], a, Qtyp q # map Styp \<gamma>)|p Z a q \<gamma>. (q, \<gamma>) \<in> delta M p a Z};
-    \<E> = {([Qtyp p, Styp Z], Qtyp q # map Styp \<gamma>)|p Z q \<gamma>. 
-        (q, \<gamma>) \<in> delta_eps M p Z} \<union> {([Q'typ q\<^sub>0], [Qtyp (init_state M), Styp (init_symbol M)])}
-        \<union> {([Qtyp f], [Q'typ q\<^sub>f])|f. f \<in> final_states M}
-  in \<lparr>states = Qtyp ` Q\<^sub>M \<union> Styp ` \<Gamma> \<union> Q'typ ` {q\<^sub>0, q\<^sub>f}, init = Q'typ q\<^sub>0, final = {Q'typ q\<^sub>f}, nxt = \<Delta>, eps = \<E>\<rparr> "
-
-lemma states_gpda_of_pda [simp]:
-  "states ((gpda_of_pda M)::(('q, 's, 'r::fresh0) sum3, 'a) gpda) 
-    = (let  q\<^sub>0 = fresh0 ({}::'r set);
-      q\<^sub>f = fresh0 {q\<^sub>0} in 
-    (Qtyp ` (UNIV :: 'q set)) \<union> (Styp ` (UNIV :: 's set)) \<union> (Q'typ ` {q\<^sub>0, q\<^sub>f}))"
-  unfolding gpda_of_pda_def by (meson gpda.select_convs(1))
-
-lemma gpda_of_pda_states_contain_pda_states_stack:
-  "Qtyp ` UNIV \<union> Styp ` UNIV \<subseteq> states (gpda_of_pda M)"
-  using states_gpda_of_pda by (metis sup_ge1)
-
-lemma init_gpda_of_pda [simp]:
-  "init ((gpda_of_pda M)::(('q, 's, 'r::fresh0) sum3, 'a) gpda) 
-    = Q'typ (fresh0 ({}::'r set))"
-  unfolding gpda_of_pda_def by (meson gpda.select_convs(2))
-
-lemma final_gpda_of_pda[simp]:
-  "final ((gpda_of_pda M)::(('q, 's, 'r::fresh0) sum3, 'a) gpda)
-    = {Q'typ (fresh0 {fresh0 ({}::'r set)})}"
-  unfolding gpda_of_pda_def by (meson gpda.select_convs(3))
-
-lemma nxt_gpda_of_pda[simp]:
-  "nxt (gpda_of_pda M) = 
-    {([Qtyp p, Styp Z], a, Qtyp q # map Styp \<gamma>)|p Z a q \<gamma>. (q, \<gamma>) \<in> delta M p a Z}"
-  unfolding gpda_of_pda_def by (meson gpda.select_convs(4))
-
-definition delta_rel :: "('q, 'a, 's) pda \<Rightarrow> ('q \<times> 's \<times> 'a \<times> 'q \<times> 's list) set" where
-  "delta_rel M \<equiv> {(p, Z, a, q, \<gamma>)|p Z a q \<gamma>. (q, \<gamma>) \<in> delta M p a Z}"
-
-lemma pda_imp_finite_delta_rel:
-  assumes "pda M"
-  shows "finite (delta_rel M)"
-proof -
-  have "delta_rel M \<subseteq> UNIV \<times> UNIV \<times> UNIV \<times> (\<Union>p a Z. delta M p a Z)"
-    (is "_ \<subseteq> _ \<times> _ \<times> _ \<times> _ ?Un")
-    unfolding delta_rel_def by fast
-  moreover from pda.finite_delta[OF assms] have "finite ?Un"
-    by simp
-  ultimately show ?thesis 
-    by (meson finite_SigmaI finite_UNIV finite_subset)
-qed
-
-lemma bij_betw_delta_rel_gpda_of_pda_nxt:
-  "bij_betw (\<lambda>(p, Z, a, q, \<gamma>). ([Qtyp p, Styp Z], a, Qtyp q # map Styp \<gamma>)) 
-    (delta_rel M) (nxt (gpda_of_pda M))"
-  (is "bij_betw ?f _ _")
-proof -
-  have "inj_on ?f (delta_rel M)"
-    by standard (auto, metis list.inj_map_strong sum3.inject(2))
-  moreover have "?f ` (delta_rel M) = (nxt (gpda_of_pda M))"
-    unfolding delta_rel_def nxt_gpda_of_pda by (standard; standard) force+
-  ultimately show ?thesis unfolding bij_betw_def by presburger
-qed
-
-
-lemma eps_gpda_of_pda[simp]:
-  "eps ((gpda_of_pda M)::(('q, 's, 'r::fresh0) sum3, 'a) gpda) = 
-  (let  q\<^sub>0 = fresh0 ({}::'r set);
-        q\<^sub>f = fresh0 {q\<^sub>0} in 
-    {([Qtyp p, Styp Z], Qtyp q # map Styp \<gamma>)|p Z q \<gamma>. 
-        (q, \<gamma>) \<in> delta_eps M p Z} \<union> {([Q'typ q\<^sub>0], [Qtyp (init_state M), Styp (init_symbol M)])}
-        \<union> {([Qtyp f], [Q'typ q\<^sub>f])|f. f \<in> final_states M})"
-  unfolding gpda_of_pda_def by (meson gpda.select_convs(5))
-
-
-lemma gpda_of_pda_nxt_imp_two:
-  assumes "(ps, a, qs) \<in> nxt (gpda_of_pda M)"
-  shows "\<exists>p Z. ps = [Qtyp p, Styp Z]"
-  using assms unfolding nxt_gpda_of_pda by blast
-
-
-lemma gpda_of_pda_nxt_imp_pda_delta:
-  assumes "(ps, a, qs) \<in> nxt (gpda_of_pda M)"
-  obtains p Z q \<gamma> where "ps = [Qtyp p, Styp Z]" "qs = Qtyp q # map Styp \<gamma>" "(q, \<gamma>) \<in> delta M p a Z"
-  using assms unfolding nxt_gpda_of_pda by blast
-
-lemma
-  assumes "pda P"
-  shows "gpda (gpda_of_pda P)"
-proof (unfold_locales, goal_cases)
-  case 1
-  then show ?case using init_gpda_of_pda states_gpda_of_pda
-    by (metis Un_iff image_eqI insertCI)
-next
-  case 2
-  then show ?case using states_gpda_of_pda final_gpda_of_pda 
-    by (smt (verit, ccfv_threshold) Un_iff empty_iff image_eqI insert_iff subsetI)
-next
-  case (3 ps a qs)
-  from gpda_of_pda_nxt_imp_pda_delta[OF this] obtain p Z q \<gamma> where ps_qs_defs:
-    "ps = [Qtyp p, Styp Z]"
-    "qs = Qtyp q # map Styp \<gamma>"
-    by metis
-  hence "set qs \<subseteq> Qtyp ` UNIV \<union> Styp ` UNIV" "set ps \<subseteq> Qtyp ` UNIV \<union> Styp ` UNIV"
-    by auto
-  with ps_qs_defs show ?case 
-    using gpda_of_pda_states_contain_pda_states_stack by auto
-next
-  case (4 ps qs)
-  then show ?case \<proof>
-next
-  case 5
-  then show ?case unfolding states_gpda_of_pda 
-    by (metis finite.simps finite_UNIV finite_Un finite_imageI)
-next
-  case 6
-  then show ?case 
-    using pda_imp_finite_delta_rel[OF assms] bij_betw_delta_rel_gpda_of_pda_nxt
-      bij_betw_finite by auto
-next
-  case 7
-  then show ?case \<proof>
-qed
-
-
-theorem Cfg_imp_gpda:
-  fixes G :: "('n, 't) Cfg"
-  obtains M :: "('q, 't) gpda" where "gpda.Lang M = LangS G" 
-  \<proof>
-
 end
